riscv-coq compiles again, but requires inlined map instance in Example.v

src/Example.v
@@ -15,15 +15,15 @@ Require Import riscv.MachineWidth32.
 
 Existing Instance DefaultRiscvState.
 
-Instance FunctionRegisterFile: RegisterFileFunctions Register (word 32) := {|
-  RegisterFile := Register -> word 32;
-  getReg(rf: Register -> word 32) := rf;
-  setReg(rf: Register -> word 32)(r: Register)(v: word 32) :=
+Instance FunctionRegisterFile: RegisterFileFunctions Register word32 := {|
+  RegisterFile := Register -> word32;
+  getReg(rf: Register -> word32) := rf;
+  setReg(rf: Register -> word32)(r: Register)(v: word32) :=
     fun r' => if (Z.eqb r' r) then v else rf r';
   initialRegs := fun r => ZToReg 0;
 |}.
 
-Definition fib6_riscv: list MachineInt := [ (* TODO should be "word 32", not MachineInt *)
+Definition fib6_riscv: list MachineInt := [ (* TODO should be "word32", not MachineInt *)
   Ox"00600993";         (* li s3,6 *)
   Ox"00000a13";         (* li s4,0 *)
   Ox"00100913";         (* li s2,1 *)
@@ -53,8 +53,94 @@ Goal False.
   (* decoder seems to work :) *)
 Abort.
 
-Definition RiscvMachine := riscv.RiscvMachine.RiscvMachine Register (word 32) Empty_set.
-Definition RiscvMachineL := riscv.RiscvMachine.RiscvMachine Register (word 32) LogEvent.
+Local Set Primitive Projections.
+Require Import coqutil.Macros.subst coqutil.Macros.unique coqutil.Map.Interface.
+Require Coq.Lists.List.
+Require Coq.Logic.Eqdep_dec.
+
+(* TODO: move me? *)
+Definition minimize_eq_proof{A: Type}(eq_dec: forall (x y: A), {x = y} + {x <> y}){x y: A}    (pf: x = y): x = y :=
+  match eq_dec x y with
+  | left p => p
+  | right n => match n pf: False with end
+  end.
+
+Module Import parameters.
+  Local Set Primitive Projections.
+  Class parameters := {
+    key : Type;
+    value : Type;
+    key_eqb : key -> key -> bool;
+    key_ltb : key -> key -> bool
+  }.
+End parameters. Notation parameters := parameters.parameters.
+
+Section SortedList.
+  Context {p : unique! parameters}.
+  Fixpoint put m (k:key) (v:value) : list (key * value) :=
+    match m with
+    | nil => cons (k, v) nil
+    | cons (k', v') m' =>
+      if key_eqb k k'
+      then cons (k, v) m'
+      else
+        if key_ltb k k'
+        then cons (k, v) m
+        else cons (k', v') (put m' k v)
+    end.
+  Fixpoint remove m (k:key) : list (key * value) :=
+    match m with
+    | nil => nil
+    | cons (k', v') m' =>
+      if key_eqb k k'
+      then m'
+      else
+        if key_ltb k k'
+        then m
+        else cons (k', v') (remove m' k)
+    end.
+  Fixpoint sorted (m : list (key * value)) :=
+    match m with
+    | cons (k1, _) ((cons (k2, _) m'') as m') => andb (key_ltb k1 k2) (sorted m')
+    | _ => true
+    end.
+  Record rep := { value : list (key * value) ; ok : sorted value = true }.
+  Lemma sorted_put m k v : sorted m = true -> sorted (put m k v) = true. Admitted.
+  Lemma sorted_remove m k : sorted m = true -> sorted (remove m k) = true. Admitted.
+  Definition map : map.map key parameters.value :=
+    let wrapped_put m k v := Build_rep (put (value m) k v) (minimize_eq_proof Bool.bool_dec (sorted_put _ _ _ (ok m))) in
+    let wrapped_remove m k := Build_rep (remove (value m) k) (minimize_eq_proof Bool.bool_dec (sorted_remove _ _ (ok m))) in
+    {|
+    map.rep := rep;
+    map.empty := Build_rep nil eq_refl;
+    map.get m k := match List.find (fun p => key_eqb k (fst p)) (value m) with
+                   | Some (_, v) => Some v
+                   | None => None
+                   end;
+    map.put := wrapped_put;
+    map.remove := wrapped_remove;
+    map.putmany m1 m2 := List.fold_right (fun '(k, v) m => wrapped_put m k v) m1 (value m2)
+  |}.
+End SortedList.
+
+Existing Instance map.
+
+Set Refine Instance Mode.
+Instance params: parameters := {
+    key := word32;
+    value := byte;
+    key_eqb := word.eqb;
+    key_ltb := word.ltu;
+}.
+Instance bar: Interface.map.map word32 byte := @map _.
+
+Module Test.
+  Definition emp: bar := map.empty.
+  Eval cbv in (map.get (map.put (map.put emp (word.of_Z 3) (word.of_Z 33)) (word.of_Z 3) (word.of_Z 44)) (word.of_Z 3)).
+End Test.
+
+Definition RiscvMachine := riscv.RiscvMachine.RiscvMachine Register word32 Empty_set.
+Definition RiscvMachineL := riscv.RiscvMachine.RiscvMachine Register word32 LogEvent.
 
 (* This example uses the memory only as instruction memory
    TODO make an example which uses memory to store data *)
@@ -62,15 +148,15 @@ Definition zeroedRiscvMachine: RiscvMachine := {|
   getRegs := initialRegs;
   getPc := ZToReg 0;
   getNextPc := ZToReg 4;
-  isMem a := regToZ_unsigned a <? 100;
-  getMem := zero_mem 100;
+  getMem := map.empty;
   getLog := nil;
 |}.
 
-Definition zeroedRiscvMachineL: RiscvMachineL := upgrade zeroedRiscvMachine nil.
+Definition zeroedRiscvMachineL: RiscvMachineL :=
+  upgrade zeroedRiscvMachine [(EvLoadWord 12345 (InvalidInstruction 777), [], [])].
 
 Definition initialRiscvMachineL(imem: list MachineInt): RiscvMachineL :=
-  putProgram (map (@ZToWord 32) imem) (ZToReg 0) zeroedRiscvMachineL.
+  putProgram imem (ZToReg 0) zeroedRiscvMachineL.
 
 Definition run: nat -> RiscvMachineL -> (option unit) * RiscvMachineL := run.
  (* @run BitWidths32 MachineWidth32 (OState RiscvMachineL) (OState_Monad _) _ _ _ *)
@@ -80,16 +166,16 @@ Definition fib6_L_final(fuel: nat): RiscvMachineL :=
   | (answer, state) => state
   end.
 
-Definition fib6_L_res(fuel: nat): word XLEN :=
+Definition fib6_L_res(fuel: nat): word32 :=
   (fib6_L_final fuel).(getRegs) 18.
 
-Definition fib6_L_trace(fuel: nat): list (LogItem (word 32) LogEvent) :=
+Definition fib6_L_trace(fuel: nat): list (LogItem word32 LogEvent) :=
   (fib6_L_final fuel).(getLog).
 
 (* only uncomment this if you're sure there are no admits in the computational parts,
    otherwise this will eat all your memory *)
 
-Eval cbv in (fib6_L_trace 50).
+Eval vm_compute in (fib6_L_trace 50).
 
 Lemma fib6_res_is_13_by_running_it: exists fuel, fib6_L_res fuel = ZToReg 13.
   exists 50%nat.
